add known value test

TestModels/SimpleTypes/SimpleBlob/src/SimpleBlobImpl.dfy
@@ -10,8 +10,12 @@ module SimpleBlobImpl refines AbstractSimpleTypesBlobOperations  {
   predicate GetBlobEnsuresPublicly(input: GetBlobInput, output: Result<GetBlobOutput, Error>) {
     true
   }
- method GetBlob ( config: InternalConfig,  input: GetBlobInput )
- returns (output: Result<GetBlobOutput, Error>) {
+  predicate GetBlobKnownValueTestEnsuresPublicly(input: GetBlobInput, output: Result<GetBlobOutput, Error>) {
+    true
+  }
+  method GetBlob ( config: InternalConfig,  input: GetBlobInput )
+    returns (output: Result<GetBlobOutput, Error>)
+  {
     expect input.value.Some?;
     ValidateBlobType(input.value.value);
 
@@ -23,7 +27,44 @@ module SimpleBlobImpl refines AbstractSimpleTypesBlobOperations  {
     expect res.value.value == input.value.value;
 
     return Success(res);
+  }
+
+  // This method is only used for known-value testing. See comment inside method which explains this method's purpose.
+  method GetBlobKnownValueTest ( config: InternalConfig,  input: GetBlobInput )
+    returns (output: Result<GetBlobOutput, Error>)
+  {
+    expect input.value.Some?;
+    ValidateBlobType(input.value.value);
+
+    // Known value test.
+    //
+    // The `input` variable this function was called with is not necessarily the same `input` that is referenced
+    //   within this function.
+    // ex. The transpiled code may have copied `input` by value into this function, rather than passing it by
+    //   reference. This is runtime-dependent behavior. 
+    // We cannot test the value of `input` from outside this function; it must be tested inside the 
+    //   implementation. In the example above, if the copy-by-value is incorrect, we would not know by
+    // 
+    // However, in order to validate the value of `input` from within this function, we must test against a known Dafny
+    //   value. This value cannot be passed into the function. As in the example above, this known value may also be
+    //   copied by value, and potentially suffer the same mutations described above.
+    // To validate this, we require a unique test vector that is defined in this function. This method is used in
+    //   conjunction with a single test that always passes in [0x0, 0x2, 0x4]. As a result, this `expect` validates
+    //   that the `input` referenced within this function matches the expected Dafny-defined test vector.
+    //
+    // Other than this `expect` statement, this function is the same as `GetBlob`.
+    expect input.value.value == [0x0, 0x2, 0x4];
+
+    var res := GetBlobOutput(value := input.value);
+    expect res.value.Some?;
+    ValidateBlobType(res.value.value);
+
+    // Validate values: input is the same as the output
+    expect res.value.value == input.value.value;
+
+    return Success(res);
  }
+
 
  method ValidateBlobType(input: seq<UInt.uint8>)
  {
