TestModels/SimpleTypes/SimpleBlob/test/SimpleBlobImplTest.dfy
@@ -9,6 +9,7 @@ module SimpleBlobImplTest {
     method{:test} GetBlob(){
         var client :- expect SimpleBlob.SimpleBlob();
         TestGetBlob(client);
+        TestGetBlobKnownValueTest(client);
     }
 
     method TestGetBlob(client: ISimpleTypesBlobClient)
@@ -31,4 +32,40 @@ module SimpleBlobImplTest {
         expect ret.value.UnwrapOr([0x0]) == s;
         print ret;
     }
+
+    method TestGetBlobKnownValueTest(client: ISimpleTypesBlobClient)
+      requires client.ValidState()
+      modifies client.Modifies
+      ensures client.ValidState()
+    {
+        var s: seq<UInt.uint8> := [0x0, 0x2, 0x4];
+        var convertedBlobInput: GetBlobInput := SimpleBlob.Types.GetBlobInput(value:= Some(s));
+        SimpleBlobImpl.ValidateBlobType(convertedBlobInput.value.value);
+        // Validate values of convertedBlobInput are same as input values
+        expect convertedBlobInput.value.value == s;
+
+        var ret :- expect client.GetBlobKnownValueTest(convertedBlobInput);
+
+        // Expect output of GetBlob has same value as input sequence
+        // i.e. GetBlob(GetBlobInput(seq)) == GetBlobInput(seq)
+        expect ret.value.UnwrapOr([0x0]) == convertedBlobInput.value.value;
+        // From above, GetBlobInput(seq) value == seq, so the below should be redundant
+        expect ret.value.UnwrapOr([0x0]) == s;
+        print ret;
+    }
+
+    // TODO: Add Blob tests using externs.
+    // 
+    // Runtimes often implement blobs using array-like structures. These structures may only be a "view" of a portion
+    //   of memory. However, there is a risk that this "view" is implemented incorrectly.
+    // For example, a Dafny blob of length 5 (|seq<uint8>| = 5) may be expected to be represented as an (ex.) Java
+    //   ByteSequence of length 5. The JRE may have already allocated a large memory buffer and would expect to
+    //   allocate memory from this buffer as needed. (This improves allocation speed performance.)
+    // However, if the Polymorph layer is incorrect, Polymorph may accidentally request the entire memory buffer,
+    //   rather than only 5 bytes. The problem is there is no way to verify whether this has happened from within the
+    //   Dafny layer. If Dafny has modelled itself correctly but the error is only detectable from inside the runtime,
+    //   Dafny does not understand how to interact with the generated code inside the runtime in a way to verify the
+    //   size of the blob (ByteSequence) is expected.
+    // The solution is to revisit this test suite after writing externs: https://sim.amazon.com/issues/CrypTool-4911
+    // We would write test suites using externs to validate the runtime code is behaving as expected.
 }
